Slightly improve some proofs and copy; fix line lengths

Contrasim_Set_Game.thy
@@ -48,16 +48,17 @@ for
   \<tau> :: \<open>'a\<close>
 begin
 
-fun strategy_from_mimicking_of_C :: \<open>('s \<Rightarrow> ('s set) \<Rightarrow> bool) \<Rightarrow> ('s, 'a) c_set_game_node strategy\<close>
+fun strategy_from_mimicking_of_C ::
+    \<open>('s \<Rightarrow> ('s set) \<Rightarrow> bool) \<Rightarrow> ('s, 'a) c_set_game_node strategy\<close>
   where
-
-  \<open>strategy_from_mimicking_of_C R ((DefenderSwapNode p1 Q)#play) = 
-    (AttackerNode (SOME q1 . (\<exists>q. (q \<in> Q \<and> q  \<Rightarrow>^\<tau> q1)) \<and> R q1 {p1}) {p1})\<close> |
-
-  \<open>strategy_from_mimicking_of_C R ((DefenderSimNode a p1 Q)#play) = 
-    (AttackerNode p1 (SOME Q1 . Q1 = dsuccs a Q \<and> R p1 Q1))\<close> |
- 
-  \<open>strategy_from_mimicking_of_C _ _ = undefined\<close>
+  
+    \<open>strategy_from_mimicking_of_C R ((DefenderSwapNode p1 Q)#play) = 
+      (AttackerNode (SOME q1 . (\<exists>q. (q \<in> Q \<and> q  \<Rightarrow>^\<tau> q1)) \<and> R q1 {p1}) {p1})\<close> |
+  
+    \<open>strategy_from_mimicking_of_C R ((DefenderSimNode a p1 Q)#play) = 
+      (AttackerNode p1 (SOME Q1 . Q1 = dsuccs a Q \<and> R p1 Q1))\<close> |
+   
+    \<open>strategy_from_mimicking_of_C _ _ = undefined\<close>
 
 lemma set_defender_pred_is_attacker: 
   assumes 
@@ -71,7 +72,8 @@ proof -
   from assms(1) have def_cases: 
     \<open>\<exists>p1 Q. (\<exists>a. n0 = DefenderSimNode a p1 Q) \<or> n0 = DefenderSwapNode p1 Q\<close>  
     using c_set_game_defender_node.elims(2) by blast
-  then obtain p1 Q where pQ_def: \<open>(\<exists>a. n0 = DefenderSimNode a p1 Q) \<or> n0 = DefenderSwapNode p1 Q\<close> 
+  then obtain p1 Q where
+    pQ_def: \<open>(\<exists>a. n0 = DefenderSimNode a p1 Q) \<or> n0 = DefenderSwapNode p1 Q\<close> 
     by auto
   hence \<open>\<exists>p. (hd play) = AttackerNode p Q\<close>
   proof (rule disjE)
@@ -89,10 +91,12 @@ lemma second_elem_in_play_set :
   assumes 
     \<open>(n0#play) \<in> plays (AttackerNode p0 Q0)\<close>
     \<open>c_set_game_defender_node n0\<close>
-  shows \<open>hd play \<in> set (n0 # play)\<close>
+  shows
+    \<open>hd play \<in> set (n0 # play)\<close>
 proof - 
   from assms have \<open>n0 \<noteq> AttackerNode p0 Q0\<close> by auto 
-  hence \<open>play \<in> plays (AttackerNode p0 Q0)\<close> using assms(1) plays.cases no_empty_plays by blast
+  hence \<open>play \<in> plays (AttackerNode p0 Q0)\<close>
+    using assms(1) plays.cases no_empty_plays by blast
   hence play_split: \<open>\<exists>x xs. play = x#xs\<close> using no_empty_plays
     using plays.cases by blast 
   then obtain x where x_def: \<open>\<exists>xs. play = x#xs\<close> ..
@@ -106,7 +110,8 @@ lemma def_sim_or_swap_before_atkNode:
     \<open>c_set_game_moves n0 n1\<close>
     \<open>n1 = AttackerNode p Q\<close>
   shows 
-    \<open>(\<exists>Qpred a. n0 = (DefenderSimNode a p Qpred)) \<or> (\<exists>q Ppred. n0 = (DefenderSwapNode q Ppred) \<and> Q = {q})\<close>
+    \<open>(\<exists>Qpred a. n0 = (DefenderSimNode a p Qpred)) \<or>
+    (\<exists>q Ppred. n0 = (DefenderSwapNode q Ppred) \<and> Q = {q})\<close>
 proof (cases n0 rule: c_set_game_node.exhaust)
   case (AttackerNode s T)
   hence \<open>c_set_game_moves (AttackerNode s T) (AttackerNode p Q)\<close> using assms by auto 
@@ -125,69 +130,86 @@ lemma set_game_strategy_retains_mimicking:
   assumes
     \<open>contrasimulation C\<close>
     \<open>C p0 q0\<close>
-    \<open>play \<in> plays_for_0strategy (strategy_from_mimicking_of_C (mimicking (set_lifted C))) (AttackerNode p0 {q0})\<close>
-  shows \<open>n = AttackerNode p Q \<Longrightarrow> n \<in> set play \<Longrightarrow> mimicking (set_lifted C) p Q \<close>
+    \<open>play \<in> plays_for_0strategy
+      (strategy_from_mimicking_of_C (mimicking (set_lifted C))) (AttackerNode p0 {q0})\<close>
+  shows
+    \<open>n = AttackerNode p Q \<Longrightarrow> n \<in> set play \<Longrightarrow> mimicking (set_lifted C) p Q \<close>
 proof (induct arbitrary: n p Q rule: plays_for_0strategy.induct[OF assms(3)])
   case init: 1
   hence \<open>p = p0 \<and> Q = {q0}\<close> using init.prems(1) by auto 
-  thus  \<open>mimicking (set_lifted C) p Q\<close> using assms R_is_in_mimicking_of_R set_lifted_def by simp
+  thus \<open>mimicking (set_lifted C) p Q\<close>
+    using assms R_is_in_mimicking_of_R set_lifted_def by simp
 next
   case p0moved: (2 n0 play) 
-  hence \<open>(n = strategy_from_mimicking_of_C (mimicking (set_lifted C)) (n0 # play)) \<or> (n \<in> set (n0#play))\<close> by auto
+  hence \<open>(n = strategy_from_mimicking_of_C
+    (mimicking (set_lifted C)) (n0 # play)) \<or> (n \<in> set (n0#play))\<close> by auto
   thus ?case
   proof(rule disjE)
     assume \<open>n \<in> set (n0#play)\<close>
     thus ?thesis using p0moved.prems p0moved.hyps(1,2) by blast 
   next
-    assume strat: \<open>n = strategy_from_mimicking_of_C (mimicking (set_lifted C)) (n0 # play)\<close>
-    hence \<open>(\<exists>a Qpred. n0 = DefenderSimNode a p Qpred) \<or> (\<exists>q Ppred. n0 = DefenderSwapNode q Ppred \<and> Q = {q})\<close>
-      using def_sim_or_swap_before_atkNode[OF p0moved.hyps(4), of \<open>p\<close> \<open>Q\<close>] p0moved.prems(1) by blast 
+    assume strat: \<open>n = strategy_from_mimicking_of_C
+      (mimicking (set_lifted C)) (n0 # play)\<close>
+    hence \<open>(\<exists>a Qpred. n0 = DefenderSimNode a p Qpred) \<or>
+        (\<exists>q Ppred. n0 = DefenderSwapNode q Ppred \<and> Q = {q})\<close>
+      using def_sim_or_swap_before_atkNode[OF p0moved.hyps(4), of \<open>p\<close> \<open>Q\<close>]
+        p0moved.prems(1)
+      by blast 
     thus ?case 
     proof (rule disjE)
       assume \<open>\<exists>a Qpred. n0 = DefenderSimNode a p Qpred\<close>
       then obtain a Qpred where n0_def: \<open>n0 = DefenderSimNode a p Qpred\<close> by auto
-      hence \<open>strategy_from_mimicking_of_C (mimicking (set_lifted C)) (n0#play) 
-          = AttackerNode p (SOME Q1. Q1 = dsuccs a Qpred \<and> (mimicking (set_lifted C)) p Q1)\<close> 
+      hence \<open>strategy_from_mimicking_of_C (mimicking (set_lifted C)) (n0#play)
+          = AttackerNode p (SOME Q1. Q1 = dsuccs a Qpred \<and> (mimicking (set_lifted C)) p Q1)\<close>
         using strategy_from_mimicking_of_C.simps(2) by auto
-      hence Q_def: \<open>Q = (SOME Q1. Q1 = dsuccs a Qpred \<and> (mimicking (set_lifted C)) p Q1)\<close> 
+      hence Q_def: \<open>Q = (SOME Q1. Q1 = dsuccs a Qpred \<and> (mimicking (set_lifted C)) p Q1)\<close>
         using strat by (simp add: p0moved.prems(1))
       have \<open>\<exists>ppred. hd play = (AttackerNode ppred Qpred) \<and> c_set_game_moves (hd play) n0\<close> 
         using set_defender_pred_is_attacker strategy0_plays_subset[OF p0moved.hyps(1)] 
-          assms(2,3) n0_def by force 
+          assms(2,3) n0_def by force
       then obtain ppred where ppred_def: \<open>hd play = (AttackerNode ppred Qpred)\<close> 
           and \<open>c_set_game_moves (hd play) n0\<close> by auto
       hence \<open>ppred =\<rhd>a p\<close> \<open>a \<noteq> \<tau>\<close> using n0_def by auto
       hence \<open>hd play \<in> set (n0 # play)\<close> 
-        using second_elem_in_play_set strategy0_plays_subset[OF p0moved.hyps(1)] assms(3) n0_def
+        using second_elem_in_play_set strategy0_plays_subset[OF p0moved.hyps(1)]
+          assms(3) n0_def
         by (simp add: assms(3))
-      hence \<open>mimicking (set_lifted C) ppred Qpred\<close> using p0moved.hyps(2) ppred_def by blast
+      hence \<open>mimicking (set_lifted C) ppred Qpred\<close>
+        using p0moved.hyps(2) ppred_def by blast
       hence \<open>mimicking (set_lifted C) p (dsuccs a Qpred)\<close> 
-       using \<open>ppred =\<rhd>a p\<close> assms(1,2) mimicking_of_C_guarantees_action_succ \<open>a \<noteq> \<tau>\<close> by auto
+        using \<open>ppred =\<rhd>a p\<close> assms(1,2) mimicking_of_C_guarantees_action_succ \<open>a \<noteq> \<tau>\<close>
+        by auto
       hence \<open>\<exists>Q. Q = (dsuccs a Qpred) \<and> mimicking (set_lifted C) p Q\<close> by auto
       from someI_ex[OF this] show \<open>mimicking (set_lifted C) p Q\<close> 
         unfolding Q_def
         using n0_def p0moved.hyps(4) by auto
     next
       assume \<open>(\<exists>q Ppred. n0 = DefenderSwapNode q Ppred \<and> Q = {q})\<close>
-      then obtain q Ppred where n0_def: \<open>n0 = DefenderSwapNode q Ppred\<close> and Q_def: \<open>Q = {q}\<close> 
+      then obtain q Ppred where
+          n0_def: \<open>n0 = DefenderSwapNode q Ppred\<close> and
+          Q_def: \<open>Q = {q}\<close> 
         by auto
       hence \<open>strategy_from_mimicking_of_C (mimicking (set_lifted C)) (n0#play)
-         = AttackerNode (SOME p1. (\<exists>p. p \<in> Ppred \<and> p \<Rightarrow>^\<tau> p1) \<and> (mimicking (set_lifted C)) p1 {q}) {q}\<close> 
+         = AttackerNode (SOME p1.
+            (\<exists>p. p \<in> Ppred \<and> p \<Rightarrow>^\<tau> p1) \<and> (mimicking (set_lifted C)) p1 {q}) {q}\<close> 
         using strategy_from_mimicking_of_C.simps(1) by auto
-      hence p_def: \<open>p = (SOME p1. (\<exists>p. p \<in> Ppred \<and> p \<Rightarrow>^\<tau> p1) \<and> (mimicking (set_lifted C)) p1 {q})\<close> 
+      hence p_def: \<open>p = (SOME p1.
+            (\<exists>p. p \<in> Ppred \<and> p \<Rightarrow>^\<tau> p1) \<and> (mimicking (set_lifted C)) p1 {q})\<close> 
         using strat p0moved.prems by auto
-      have \<open>\<exists>qpred. hd play = (AttackerNode qpred Ppred) \<and> c_set_game_moves (hd play) n0\<close> 
+      have \<open>\<exists>qpred. hd play = (AttackerNode qpred Ppred) \<and> c_set_game_moves (hd play) n0\<close>
         using set_defender_pred_is_attacker strategy0_plays_subset[OF p0moved.hyps(1)] 
           assms(3) n0_def
-        by force 
+        by force
       then obtain qpred where qpred_def: \<open>hd play = (AttackerNode qpred Ppred)\<close> 
         and qpred_move: \<open>c_set_game_moves (hd play) n0\<close> by auto
       hence p1: \<open>player1_position (hd play)\<close> by simp
       have qpred_q_move: \<open>qpred \<Rightarrow>^\<tau> q\<close> using qpred_def qpred_move n0_def by simp
       have \<open>hd play \<in> set (n0 # play)\<close> 
-        using second_elem_in_play_set strategy0_plays_subset[OF p0moved.hyps(1)] assms(3) n0_def
+        using second_elem_in_play_set strategy0_plays_subset[OF p0moved.hyps(1)]
+          assms(3) n0_def
         by simp 
-      hence \<open>mimicking (set_lifted C) qpred Ppred\<close> using p0moved.hyps(2) qpred_def by blast
+      hence \<open>mimicking (set_lifted C) qpred Ppred\<close>
+        using p0moved.hyps(2) qpred_def by blast
       hence \<open>\<exists>p. p \<in> weak_tau_succs Ppred \<and> mimicking (set_lifted C) p {q}\<close> 
         using qpred_q_move assms(1,2) mimicking_of_C_guarantees_tau_succ by blast
       hence \<open>\<exists>p. (\<exists>p0. p0 \<in> Ppred \<and> p0 \<Rightarrow>^\<tau>  p) \<and> mimicking (set_lifted C) p {q}\<close> 
@@ -217,16 +239,22 @@ lemma set_contrasim_game_complete:
   assumes
     \<open>contrasimulation C\<close>
     \<open>C p0 q0\<close>
-  shows \<open>player0_winning_strategy (strategy_from_mimicking_of_C (mimicking (set_lifted C))) (AttackerNode p0 {q0})\<close>
+  shows
+    \<open>player0_winning_strategy (strategy_from_mimicking_of_C
+      (mimicking (set_lifted C))) (AttackerNode p0 {q0})\<close>
   unfolding player0_winning_strategy_def
 proof (safe)
   fix play
-  assume A1: \<open>play \<in> (plays_for_0strategy (strategy_from_mimicking_of_C (mimicking (set_lifted C))) (AttackerNode p0 {q0}))\<close>
+  assume A1: \<open>play \<in> (plays_for_0strategy
+    (strategy_from_mimicking_of_C (mimicking (set_lifted C))) (AttackerNode p0 {q0}))\<close>
   thus \<open>player1_wins_immediately play \<Longrightarrow> False\<close>
     unfolding player1_wins_immediately_def
-  proof - 
-    assume A: \<open>c_set_game_defender_node (hd play) \<and> (\<nexists>p'. c_set_game_moves (hd play) p')\<close> 
-    have player0_has_succ_node: \<open>c_set_game_defender_node (hd play) \<Longrightarrow> \<exists>p'. c_set_game_moves (hd play) p'\<close>
+  proof clarify
+    assume A:
+      \<open>c_set_game_defender_node (hd play)\<close>
+      \<open>\<nexists>p'. c_set_game_moves (hd play) p'\<close> 
+    have player0_has_succ_node:
+      \<open>c_set_game_defender_node (hd play) \<Longrightarrow> \<exists>p'. c_set_game_moves (hd play) p'\<close>
     proof (induct rule: simple_game.plays_for_0strategy.induct[OF A1])
       case init: 1
       have \<open>\<not>c_set_game_defender_node (AttackerNode p0 {q0})\<close> by (simp add: assms) 
@@ -237,25 +265,30 @@ proof (safe)
       from p0moved.hyps have \<open>c_set_game_defender_node n0\<close> by simp
       hence \<open>(\<exists>a p1 q. n0 = (DefenderSimNode a p1 q)) \<or> (\<exists>q P. n0 = DefenderSwapNode q P)\<close>
         by (meson c_set_game_defender_node.elims(2)) 
-      hence \<open>\<not>c_set_game_defender_node (strategy_from_mimicking_of_C (mimicking (set_lifted C)) (n0#play))\<close>
+      hence \<open>\<not>c_set_game_defender_node (strategy_from_mimicking_of_C
+          (mimicking (set_lifted C)) (n0#play))\<close>
         using p0moved.hyps(4) 
-          c_set_game_moves.elims(2)[of \<open>n0\<close> \<open>strategy_from_mimicking_of_C (mimicking (set_lifted C)) (n0#play)\<close>]
+          c_set_game_moves.elims(2)[of \<open>n0\<close>
+            \<open>strategy_from_mimicking_of_C (mimicking (set_lifted C)) (n0#play)\<close>]
         by force 
-      hence \<open>\<not>c_set_game_defender_node (hd (strategy_from_mimicking_of_C (mimicking (set_lifted C)) (n0 # play) # n0 # play))\<close> 
+      hence \<open>\<not>c_set_game_defender_node (hd (strategy_from_mimicking_of_C
+          (mimicking (set_lifted C)) (n0 # play) # n0 # play))\<close> 
         by simp
       hence \<open>False\<close> using p0moved.prems ..
       then show ?case ..
     next
       case p1moved: (3 n1 play n1') 
-      hence \<open>\<not>c_set_game_defender_node n1\<close> using p1moved.hyps by simp
+      hence \<open>\<not>c_set_game_defender_node n1\<close>
+        using p1moved.hyps by simp
       then obtain p Q where n1_def: \<open>n1 = AttackerNode p Q\<close>
         using c_set_game_defender_node.elims(3) by auto
       hence in_mimicking: \<open>mimicking (set_lifted C) p Q\<close> 
-        using set_game_strategy_retains_mimicking[OF assms, of \<open>n1#play\<close>, OF p1moved.hyps(1)] 
+        using set_game_strategy_retains_mimicking[OF assms, of \<open>n1#play\<close>, OF p1moved.hyps(1)]
         by auto
       have \<open>(\<exists>a p1. n1' = DefenderSimNode a p1 Q) \<or> (\<exists>p1. n1' = DefenderSwapNode p1 Q)\<close> 
         using p1moved.prems n1_def p1moved.hyps(4)
-        by (metis c_set_game_defender_node.elims(2) list.sel(1) local.simulation_challenge local.swap_challenge)
+        by (metis c_set_game_defender_node.elims(2) list.sel(1)
+            local.simulation_challenge local.swap_challenge)
       thus ?case
       proof (rule disjE)
         assume A: \<open>\<exists>a p1. n1' = DefenderSimNode a p1 Q\<close>
@@ -289,46 +322,59 @@ proof (safe)
   qed
 qed
 
-lemma strategy_from_mimicking_of_C_sound : 
+lemma strategy_from_mimicking_of_C_sound:
   assumes
     \<open>contrasimulation C\<close>
     \<open>C p0 q0\<close>
   shows
-    \<open>sound_0strategy (strategy_from_mimicking_of_C (mimicking (set_lifted C))) (AttackerNode p0 {q0})\<close>
+    \<open>sound_0strategy
+      (strategy_from_mimicking_of_C (mimicking (set_lifted C)))
+      (AttackerNode p0 {q0})\<close>
   unfolding sound_0strategy_def
 proof (safe)
   fix n0 play
-  assume A: 
-    \<open>n0 # play \<in> plays_for_0strategy (strategy_from_mimicking_of_C (mimicking (set_lifted C))) (AttackerNode p0 {q0})\<close>
+  assume A:
+    \<open>n0 # play \<in> plays_for_0strategy
+      (strategy_from_mimicking_of_C (mimicking (set_lifted C))) (AttackerNode p0 {q0})\<close>
     \<open>c_set_game_defender_node n0\<close>
   hence \<open>(\<exists>a p' Q. n0 = DefenderSimNode a p' Q) \<or> (\<exists>p' Q. n0 = DefenderSwapNode p' Q)\<close>
     by (meson c_set_game_defender_node.elims(2))
-  thus \<open>c_set_game_moves n0 (strategy_from_mimicking_of_C (mimicking (set_lifted C)) (n0 # play))\<close>
+  thus \<open>c_set_game_moves n0
+    (strategy_from_mimicking_of_C (mimicking (set_lifted C)) (n0 # play))\<close>
   proof(rule disjE)
     assume \<open>\<exists>a p' Q. n0 = DefenderSimNode a p' Q\<close>
     then obtain a p' Q where n0_def: \<open>n0 = DefenderSimNode a p' Q\<close> by auto
-    then obtain p where p_def: \<open>hd play = AttackerNode p Q\<close> using A
-      by (metis set_defender_pred_is_attacker simulation_challenge strategy0_plays_subset) 
+    then obtain p where p_def: \<open>hd play = AttackerNode p Q\<close>
+      using A
+      by (metis set_defender_pred_is_attacker simulation_challenge strategy0_plays_subset)
     hence \<open>c_set_game_moves (AttackerNode p Q) (DefenderSimNode a p' Q)\<close>
-      by (metis A n0_def set_defender_pred_is_attacker strategy0_plays_subset) 
-    hence \<open>p =\<rhd>a p'\<close> \<open>\<not> tau a\<close> by auto   
+      by (metis A n0_def set_defender_pred_is_attacker strategy0_plays_subset)
+    hence \<open>p =\<rhd>a p'\<close> \<open>\<not> tau a\<close> by auto
     hence \<open>mimicking (set_lifted C) p Q\<close>
       using set_game_strategy_retains_mimicking[OF assms] A p_def
-        assms(2) second_elem_in_play_set strategy0_plays_subset 
+        assms(2) second_elem_in_play_set strategy0_plays_subset
       by fastforce
     hence  \<open>mimicking (set_lifted C) p' (dsuccs a Q)\<close>
-      using mimicking_of_C_guarantees_action_succ \<open>\<not> tau a\<close> \<open>p =\<rhd>a p'\<close> assms(1) tau_tau by blast 
+      using mimicking_of_C_guarantees_action_succ \<open>\<not> tau a\<close> \<open>p =\<rhd>a p'\<close> assms(1) tau_tau
+      by blast 
     hence Q1_ex: \<open>\<exists>Q'. Q' = dsuccs a Q \<and> mimicking (set_lifted C) p' Q'\<close> by auto
-    from n0_def have st: \<open>strategy_from_mimicking_of_C (mimicking (set_lifted C)) (n0#play) = 
-    (AttackerNode p' (SOME Q1 . Q1 = dsuccs a Q \<and> (mimicking (set_lifted C)) p' Q1))\<close> by auto
+    from n0_def have st:
+      \<open>strategy_from_mimicking_of_C (mimicking (set_lifted C)) (n0#play)
+      = (AttackerNode p'
+          (SOME Q1 . Q1 = dsuccs a Q \<and> (mimicking (set_lifted C)) p' Q1))\<close>
+      by auto
     then obtain Q1 where 
-      \<open>AttackerNode p' (SOME Q1 . Q1 = dsuccs a Q \<and> (mimicking (set_lifted C)) p' Q1) = AttackerNode p' Q1\<close>
+      \<open>AttackerNode p' (SOME Q1 . Q1 = dsuccs a Q \<and> (mimicking (set_lifted C)) p' Q1)
+        = AttackerNode p' Q1\<close>
       by blast
     hence Q1_def: \<open>Q1 = (SOME Q1 . Q1 = dsuccs a Q \<and> (mimicking (set_lifted C)) p' Q1)\<close>
       by auto
-    have next_is_atk: \<open>strategy_from_mimicking_of_C (mimicking (set_lifted C)) (n0#play) = (AttackerNode p' Q1)\<close> 
+    have next_is_atk:
+      \<open>strategy_from_mimicking_of_C (mimicking (set_lifted C)) (n0#play)
+      = (AttackerNode p' Q1)\<close> 
       using st Q1_def by auto
-    with someI_ex[OF Q1_ex] Q1_def have mov_cond: \<open>Q1 = dsuccs a Q \<and> mimicking (set_lifted C) p' Q1\<close>
+    with someI_ex[OF Q1_ex] Q1_def
+      have mov_cond: \<open>Q1 = dsuccs a Q \<and> mimicking (set_lifted C) p' Q1\<close>
       by blast
     have \<open>c_set_game_moves n0 (AttackerNode p' Q1)\<close> using n0_def mov_cond by auto
     thus ?thesis using next_is_atk by auto
@@ -346,31 +392,38 @@ proof (safe)
       by fastforce 
     hence  \<open>\<exists>q'. q' \<in> weak_tau_succs Q \<and> mimicking (set_lifted C) q' {p'}\<close>
       using mimicking_of_C_guarantees_tau_succ \<open>p \<Rightarrow>^\<tau> p'\<close> assms(1) by auto 
-    hence q1_ex: \<open>\<exists>q1. (\<exists>q.(q \<in> Q \<and> q  \<Rightarrow>^\<tau> q1)) \<and> mimicking (set_lifted C) q1 {p'}\<close> using weak_tau_succs_def by auto
-    hence strat: \<open>strategy_from_mimicking_of_C (mimicking (set_lifted C)) (n0#play) = 
-    AttackerNode (SOME q1 . (\<exists>q. (q \<in> Q \<and> q  \<Rightarrow>^\<tau> q1)) \<and> (mimicking (set_lifted C)) q1 {p'}) {p'}\<close>
+    hence q1_ex: \<open>\<exists>q1. (\<exists>q.(q \<in> Q \<and> q  \<Rightarrow>^\<tau> q1)) \<and> mimicking (set_lifted C) q1 {p'}\<close>
+      using weak_tau_succs_def by auto
+    hence strat: \<open>strategy_from_mimicking_of_C (mimicking (set_lifted C)) (n0#play)
+      = AttackerNode (SOME q1.
+        (\<exists>q. (q \<in> Q \<and> q  \<Rightarrow>^\<tau> q1)) \<and> (mimicking (set_lifted C)) q1 {p'}) {p'}\<close>
       using n0_def by auto
     then obtain q1 where 
-      \<open>AttackerNode (SOME q1 . (\<exists>q. (q \<in> Q \<and> q  \<Rightarrow>^\<tau> q1)) \<and> (mimicking (set_lifted C)) q1 {p'}) {p'}
+      \<open>AttackerNode (SOME q1.
+        (\<exists>q. (q \<in> Q \<and> q  \<Rightarrow>^\<tau> q1)) \<and> (mimicking (set_lifted C)) q1 {p'}) {p'}
       = AttackerNode q1 {p'}\<close> by blast
-    hence q1_def: \<open>q1 = (SOME q1 . (\<exists>q. (q \<in> Q \<and> q  \<Rightarrow>^\<tau> q1)) \<and> (mimicking (set_lifted C)) q1 {p'})\<close>
+    hence q1_def:
+      \<open>q1 = (SOME q1 . (\<exists>q. (q \<in> Q \<and> q  \<Rightarrow>^\<tau> q1)) \<and> (mimicking (set_lifted C)) q1 {p'})\<close>
       by auto
-    with someI_ex[OF q1_ex] have X: \<open>\<exists>q. (q \<in> Q \<and> q  \<Rightarrow>^\<tau> q1) \<and> mimicking (set_lifted C) q1 {p'}\<close> 
+    with someI_ex[OF q1_ex] have X:
+      \<open>\<exists>q. (q \<in> Q \<and> q  \<Rightarrow>^\<tau> q1) \<and> mimicking (set_lifted C) q1 {p'}\<close> 
       by blast
-    hence \<open>q1 \<in> weak_tau_succs Q \<and> {p'} = {p'}\<close>using weak_tau_succs_def by auto
+    hence \<open>q1 \<in> weak_tau_succs Q \<and> {p'} = {p'}\<close>
+      using weak_tau_succs_def by auto
     thus ?thesis  using n0_def strat q1_def by auto
   qed
 qed
 
 subsection \<open>Winning Strategy Implies Contrasimulation (Soundness)\<close>
 
-lemma move_DefSim_to_AtkNode : 
+lemma move_DefSim_to_AtkNode:
   assumes 
     \<open>c_set_game_moves (DefenderSimNode a p Q) n0\<close>
-  shows \<open>n0 = AttackerNode p (dsuccs a Q)\<close>
+  shows
+    \<open>n0 = AttackerNode p (dsuccs a Q)\<close>
 proof - 
   have \<open>\<exists>p1 Q1. n0 = AttackerNode p1 Q1\<close>
-    by (metis assms c_set_game_defender_node.elims(2, 3) local.c_set_game_moves_no_step(1, 6))
+    by (metis assms c_set_game_defender_node.elims(2, 3) c_set_game_moves_no_step(1, 6))
   then obtain p1 Q1 where n0_def: \<open>n0 = AttackerNode p1 Q1\<close> by auto
   hence \<open>p = p1\<close> using assms local.simulation_answer by blast 
   from n0_def have \<open>Q1 = dsuccs a Q\<close> 
@@ -378,10 +431,11 @@ proof -
   thus ?thesis using \<open>p = p1\<close> n0_def by auto
 qed
 
-lemma move_DefSwap_to_AtkNode : 
+lemma move_DefSwap_to_AtkNode:
   assumes 
     \<open>c_set_game_moves (DefenderSwapNode p' Q) n0\<close>
-  shows \<open>\<exists>q'. n0 = AttackerNode q' {p'} \<and> q' \<in> weak_tau_succs Q\<close>
+  shows
+    \<open>\<exists>q'. n0 = AttackerNode q' {p'} \<and> q' \<in> weak_tau_succs Q\<close>
 proof - 
   have \<open>\<not>c_set_game_defender_node n0\<close> 
     using assms c_set_game_moves_no_step(3, 4) c_set_game_defender_node.elims(2)
@@ -394,7 +448,6 @@ proof -
   thus ?thesis using  \<open>P1 = {p'}\<close> n0_def by simp
 qed
 
-
 lemma def_never_stuck_on_sim_pos: 
   assumes \<open>n0 = DefenderSimNode a p Q\<close>
   shows \<open>\<exists>Q'. c_set_game_moves n0 (AttackerNode p Q')\<close>
@@ -402,7 +455,6 @@ proof -
   have \<open>c_set_game_moves (DefenderSimNode a p Q) (AttackerNode p (dsuccs a Q))\<close> by auto
   thus ?thesis using assms by auto
 qed
-
 
 lemma def_sim_pos_with_prefix_in_play: 
   assumes 
@@ -412,61 +464,88 @@ lemma def_sim_pos_with_prefix_in_play:
     \<open>sound_0strategy f (AttackerNode p00 {q00})\<close>
     \<open>play \<in> plays_for_0strategy f (AttackerNode p00 {q00})\<close>
     \<open>hd play = AttackerNode p {q}\<close>
-  shows \<open>\<exists>play p0. ((DefenderSimNode (last A) p0 (dsuccs_seq_rec (rev (butlast A)) {q}))#play) 
-      \<in> plays_for_0strategy f (AttackerNode p00 {q00}) \<and> word_reachable_via_delay A p p0 p1\<close> using assms(1-3)
-proof (induct arbitrary:  p1 rule: rev_nonempty_induct[OF assms(1)])
+  shows
+    \<open>\<exists>play p0.
+      ((DefenderSimNode (last A) p0 (dsuccs_seq_rec (rev (butlast A)) {q}))#play)
+        \<in> plays_for_0strategy f (AttackerNode p00 {q00})
+      \<and> word_reachable_via_delay A p p0 p1\<close>
+  using assms(1-3)
+proof (induct arbitrary: p1 rule: rev_nonempty_induct[OF assms(1)])
   case single: (1 a)
   hence \<open>\<not>tau a\<close> using \<open>\<forall>a\<in>set A. a \<noteq> \<tau>\<close> by (simp add: tau_def) 
   hence \<open>p \<Rightarrow>$[a] p1\<close> using single by auto
   hence p_step: \<open>p \<Rightarrow>^a p1\<close> by blast
   then obtain p0 where \<open>p =\<rhd>a p0\<close> \<open>p0 \<Rightarrow>^\<tau> p1\<close> using Cons \<open>\<not>tau a\<close> steps.refl by auto
-  hence \<open>\<exists>n0. n0  = DefenderSimNode a p0 {q} \<and> c_set_game_moves (AttackerNode p {q}) n0\<close> 
+  hence \<open>\<exists>n0. n0  = DefenderSimNode a p0 {q} \<and> c_set_game_moves (AttackerNode p {q}) n0\<close>
     using assms(4) \<open>\<not> tau a\<close> by simp
-  hence  \<open>((DefenderSimNode a p0 {q})#play) \<in> plays_for_0strategy f (AttackerNode p00 {q00})\<close> using assms(5,6)
+  hence \<open>(DefenderSimNode a p0 {q})#play \<in> plays_for_0strategy f (AttackerNode p00 {q00})\<close>
+    using assms(5,6)
     by (metis c_set_game_defender_node.simps(1) list.collapse no_empty_plays 
           plays_for_0strategy.p1move strategy0_plays_subset)
-  hence inplay: \<open>((DefenderSimNode (last [a]) p0  (dsuccs_seq_rec (rev (butlast [a])) {q}))#play) \<in> plays_for_0strategy f (AttackerNode p00 {q00})\<close>
+  hence inplay:
+    \<open>(DefenderSimNode (last [a]) p0 (dsuccs_seq_rec (rev (butlast [a])) {q}))#play
+      \<in> plays_for_0strategy f (AttackerNode p00 {q00})\<close>
     by auto
   have \<open>p  \<Rightarrow>$(butlast [a]) p\<close> by (simp add: steps.refl) 
-  hence \<open>word_reachable_via_delay [a] p p0 p1\<close> using word_reachable_via_delay_def \<open>p =\<rhd>a p0\<close> \<open>p0 \<Rightarrow>^\<tau> p1\<close> by auto
+  hence \<open>word_reachable_via_delay [a] p p0 p1\<close>
+    using word_reachable_via_delay_def \<open>p =\<rhd>a p0\<close> \<open>p0 \<Rightarrow>^\<tau> p1\<close> by auto
   then show ?case using inplay by auto
 next
   case snoc: (2 a as)
   hence \<open>\<not>tau a\<close> using \<open>\<forall>a\<in>set A. a \<noteq> \<tau>\<close> by (simp add: tau_def) 
-  then obtain a2 as2 where as_def: \<open>as = as2@[a2]\<close> using list_rev_split[OF snoc.hyps(1)] by auto
-  have \<open>\<exists>p'. p \<Rightarrow>$ as  p' \<and> p' \<Rightarrow>$[a]  p1\<close> using rev_seq_split[OF snoc.prems(2)] by blast
+  then obtain a2 as2 where as_def: \<open>as = as2@[a2]\<close>
+    using list_rev_split[OF snoc.hyps(1)] by auto
+  have \<open>\<exists>p'. p \<Rightarrow>$ as  p' \<and> p' \<Rightarrow>$[a]  p1\<close>
+    using rev_seq_split[OF snoc.prems(2)] by blast
   hence \<open>\<exists>p'. p \<Rightarrow>$ as  p' \<and> p' \<Rightarrow>^a  p1\<close> by blast
   hence \<open>\<exists>p'. p \<Rightarrow>$ as  p' \<and> p' \<Rightarrow>a  p1\<close> using  \<open>\<not>tau a\<close> by simp
   then obtain p' where p'_def: \<open>p \<Rightarrow>$ as  p'\<close> and p'_step: \<open>p' \<Rightarrow>a  p1\<close> by auto
-  then obtain p11 where  \<open>p' =\<rhd>a  p11\<close> \<open>p11 \<Rightarrow>^\<tau> p1\<close> using steps.refl \<open>\<not> tau a\<close> tau_tau by blast
+  then obtain p11 where  \<open>p' =\<rhd>a  p11\<close> \<open>p11 \<Rightarrow>^\<tau> p1\<close>
+    using steps.refl \<open>\<not> tau a\<close> tau_tau by blast
   hence \<open>\<exists>play p0.
-     DefenderSimNode (last as) p0 (dsuccs_seq_rec (rev (butlast as)) {q}) # play
-     \<in> plays_for_0strategy f (AttackerNode p00 {q00}) \<and> word_reachable_via_delay as p p0 p'\<close>  using p'_def snoc by auto
+    DefenderSimNode (last as) p0 (dsuccs_seq_rec (rev (butlast as)) {q}) # play
+      \<in> plays_for_0strategy f (AttackerNode p00 {q00})
+    \<and> word_reachable_via_delay as p p0 p'\<close>
+    using p'_def snoc by auto
   then obtain play p0
-    where play_def: \<open>DefenderSimNode (last as) p0 (dsuccs_seq_rec (rev (butlast as)) {q}) # play
-     \<in> plays_for_0strategy f (AttackerNode p00 {q00})\<close> \<open>word_reachable_via_delay as p p0 p'\<close> by auto
-
-  hence \<open>DefenderSimNode a2 p0 (dsuccs_seq_rec (rev as2) {q}) # play 
-              \<in> plays_for_0strategy f (AttackerNode p00 {q00})\<close> using as_def by auto
-  then obtain n0 where n0_def: \<open>n0 = DefenderSimNode a2 p0 (dsuccs_seq_rec (rev as2) {q})\<close> 
-        and n0_in_play: \<open>n0#play \<in> plays_for_0strategy f (AttackerNode p00 {q00})\<close> by auto
-  then obtain n1 
-    where n1_def: \<open>c_set_game_moves (DefenderSimNode a2 p0 (dsuccs_seq_rec (rev as2) {q})) n1\<close> 
+    where play_def:
+      \<open>DefenderSimNode (last as) p0 (dsuccs_seq_rec (rev (butlast as)) {q}) # play
+        \<in> plays_for_0strategy f (AttackerNode p00 {q00})\<close>
+      \<open>word_reachable_via_delay as p p0 p'\<close>
+    by auto
+  hence
+    \<open>DefenderSimNode a2 p0 (dsuccs_seq_rec (rev as2) {q}) # play
+      \<in> plays_for_0strategy f (AttackerNode p00 {q00})\<close>
+    using as_def by auto
+  then obtain n0 where
+    n0_def: \<open>n0 = DefenderSimNode a2 p0 (dsuccs_seq_rec (rev as2) {q})\<close> and
+    n0_in_play: \<open>n0#play \<in> plays_for_0strategy f (AttackerNode p00 {q00})\<close>
+    by auto
+  then obtain n1 where
+    n1_def: \<open>c_set_game_moves (DefenderSimNode a2 p0 (dsuccs_seq_rec (rev as2) {q})) n1\<close>
     using def_never_stuck_on_sim_pos by meson
-  hence n1_atk: \<open>n1 = AttackerNode p0 (dsuccs a2 ((dsuccs_seq_rec (rev as2) {q})))\<close> 
+  hence n1_atk: \<open>n1 = AttackerNode p0 (dsuccs a2 ((dsuccs_seq_rec (rev as2) {q})))\<close>
     using move_DefSim_to_AtkNode[OF n1_def] by auto
-  have n1_in_play: \<open>n1#n0#play \<in> plays_for_0strategy f (AttackerNode p00 {q00})\<close> using n1_def n0_in_play n0_def
-    by (metis assms(4) move_DefSim_to_AtkNode c_set_game_defender_node.simps(2) 
-        plays_for_0strategy.simps sound_0strategy_def) 
-  then obtain n0' 
-    where n0'_def : \<open>n0' = DefenderSimNode a p11 (dsuccs a2 ((dsuccs_seq_rec (rev as2) {q})))\<close> 
-    and n0'_mov: \<open>c_set_game_moves n1 n0'\<close> using p'_step n1_atk
-    by (metis (no_types, lifting) \<open>\<not> tau a\<close> \<open>p' =\<rhd> a p11\<close> word_reachable_via_delay_def simulation_challenge play_def(2) steps_concat tau_tau)
-  hence in_play: \<open>n0'#n1#n0#play \<in> plays_for_0strategy f (AttackerNode p00 {q00})\<close> using n1_in_play
+  have n1_in_play: \<open>n1#n0#play \<in> plays_for_0strategy f (AttackerNode p00 {q00})\<close>
+    using n1_def n0_in_play n0_def
+    by (metis assms(4) move_DefSim_to_AtkNode c_set_game_defender_node.simps(2)
+        plays_for_0strategy.simps sound_0strategy_def)
+  then obtain n0' where
+    n0'_def:
+      \<open>n0' = DefenderSimNode a p11 (dsuccs a2 ((dsuccs_seq_rec (rev as2) {q})))\<close> and
+    n0'_mov: \<open>c_set_game_moves n1 n0'\<close>
+    using p'_step n1_atk
+    by (metis (no_types, lifting) \<open>\<not> tau a\<close> \<open>p' =\<rhd> a p11\<close> word_reachable_via_delay_def
+        simulation_challenge play_def(2) steps_concat tau_tau)
+  hence in_play: \<open>n0'#n1#n0#play \<in> plays_for_0strategy f (AttackerNode p00 {q00})\<close>
+    using n1_in_play
     by (simp add: n1_atk plays_for_0strategy.p1move) 
-  hence \<open>n0' = DefenderSimNode a p11 (dsuccs_seq_rec (rev (as2@[a2])) {q})\<close> using n0'_def  by auto
-  hence n0'_is_defSimNode: \<open>n0' = DefenderSimNode a p11 (dsuccs_seq_rec (rev (as)) {q})\<close> using as_def by auto
-  from \<open>p \<Rightarrow>$ as  p'\<close> \<open>p' =\<rhd>a  p11\<close> \<open>p11 \<Rightarrow>^\<tau> p1\<close> have \<open>word_reachable_via_delay (as@[a]) p p11 p1\<close> 
+  hence \<open>n0' = DefenderSimNode a p11 (dsuccs_seq_rec (rev (as2@[a2])) {q})\<close>
+    using n0'_def  by auto
+  hence n0'_is_defSimNode: \<open>n0' = DefenderSimNode a p11 (dsuccs_seq_rec (rev (as)) {q})\<close>
+    using as_def by auto
+  from \<open>p \<Rightarrow>$ as  p'\<close> \<open>p' =\<rhd>a  p11\<close> \<open>p11 \<Rightarrow>^\<tau> p1\<close>
+    have \<open>word_reachable_via_delay (as@[a]) p p11 p1\<close> 
     using word_reachable_via_delay_def by auto
   then show ?case using n0'_is_defSimNode in_play by auto
 qed
@@ -480,40 +559,53 @@ lemma set_contrasim_game_sound:
       hd play = AttackerNode p {q} \<and> (hd play = (AttackerNode p00 {q00})
       \<or> (\<exists>P. hd (tl play) = DefenderSwapNode q P)))\<close>
   shows
-    \<open>contrasimulation C\<close>  unfolding contrasimulation_def
+    \<open>contrasimulation C\<close>
+  unfolding contrasimulation_def
 proof (safe) 
   fix p q p1 A
-  assume \<open>\<forall>a\<in>set A. a \<noteq> \<tau>\<close> \<open>p \<Rightarrow>$A p1\<close> and \<open>C p q\<close> 
+  assume \<open>\<forall>a\<in>set A. a \<noteq> \<tau>\<close> \<open>p \<Rightarrow>$A p1\<close> \<open>C p q\<close>
   hence \<open>p \<Rightarrow>$(taufree A) p1\<close> by (simp add: weak_step_over_tau) 
-  hence \<open>(\<exists> play \<in> plays_for_0strategy f (AttackerNode p00 {q00}). hd play = AttackerNode p {q} \<and> (hd play = (AttackerNode p00 {q00}) \<or> (\<exists>P. hd (tl play) = DefenderSwapNode q P)))\<close> 
-    using C_def \<open>p \<Rightarrow>$A p1\<close> and \<open>C p q\<close>  by auto
-  from this obtain play where play_def: \<open>play \<in> plays_for_0strategy f (AttackerNode p00 {q00})\<close> 
-    and play_hd: \<open>hd play = AttackerNode p {q}\<close> 
-    and \<open>hd play = (AttackerNode p00 {q00}) \<or> (\<exists>P. hd (tl play) = DefenderSwapNode q P)\<close> 
+  hence \<open>\<exists> play \<in> plays_for_0strategy f (AttackerNode p00 {q00}).
+      hd play = AttackerNode p {q}
+      \<and> (hd play = (AttackerNode p00 {q00})
+      \<or> (\<exists>P. hd (tl play) = DefenderSwapNode q P))\<close>
+    using C_def \<open>p \<Rightarrow>$A p1\<close> \<open>C p q\<close> by auto
+  from this obtain play where
+    play_def: \<open>play \<in> plays_for_0strategy f (AttackerNode p00 {q00})\<close> and
+    play_hd: \<open>hd play = AttackerNode p {q}\<close> and
+    \<open>hd play = (AttackerNode p00 {q00}) \<or> (\<exists>P. hd (tl play) = DefenderSwapNode q P)\<close> 
     by auto
-  hence \<open>\<not>player1_wins_immediately play\<close> using assms(1) player0_winning_strategy_def by auto
-  hence \<open>(c_set_game_defender_node (hd play) \<and> (\<nexists>p'. c_set_game_moves (hd play) p')) \<Longrightarrow> False\<close> 
+  hence \<open>\<not>player1_wins_immediately play\<close>
+    using assms(1) player0_winning_strategy_def by auto
+  hence \<open>(c_set_game_defender_node (hd play) \<and>
+    (\<nexists>p'. c_set_game_moves (hd play) p')) \<Longrightarrow> False\<close> 
     using player1_wins_immediately_def by auto
-  hence Def_not_stuck: \<open>c_set_game_defender_node (hd play) \<Longrightarrow> (\<exists>p'. c_set_game_moves (hd play) p')\<close> by auto
-  from \<open>p \<Rightarrow>$A p1\<close> \<open>p \<Rightarrow>$(taufree A) p1\<close> \<open>C p q\<close> show \<open>\<exists>q'. q \<Rightarrow>$ A q' \<and> C q' p1\<close>
+  hence Def_not_stuck:
+    \<open>c_set_game_defender_node (hd play) \<Longrightarrow> (\<exists>p'. c_set_game_moves (hd play) p')\<close> by auto
+  from \<open>p \<Rightarrow>$A p1\<close> \<open>p \<Rightarrow>$(taufree A) p1\<close> \<open>C p q\<close>
+    show \<open>\<exists>q'. q \<Rightarrow>$ A q' \<and> C q' p1\<close>
   proof (cases A rule: rev_cases)
     case Nil
     hence \<open>p \<Rightarrow>^\<tau> p1\<close> using \<open>p \<Rightarrow>$A p1\<close> by auto
-    hence \<open>\<exists>n0. n0 = DefenderSwapNode p1 {q} \<and> c_set_game_moves (AttackerNode p {q}) n0\<close> by simp 
+    hence \<open>\<exists>n0. n0 = DefenderSwapNode p1 {q}
+      \<and> c_set_game_moves (AttackerNode p {q}) n0\<close> by simp 
     from this obtain n0 where n0_def: \<open>n0 = DefenderSwapNode p1 {q}\<close> 
       and n0_move: \<open>c_set_game_moves (AttackerNode p {q}) n0\<close> by auto
     have \<open>play = (hd play)#(tl play)\<close>
       by (metis hd_Cons_tl no_empty_plays play_def strategy0_plays_subset)
-    hence \<open>n0#play \<in> plays_for_0strategy f (AttackerNode p00 {q00})\<close> using n0_def n0_move play_def play_hd
+    hence \<open>n0#play \<in> plays_for_0strategy f (AttackerNode p00 {q00})\<close>
+      using n0_def n0_move play_def play_hd
       by (metis c_set_game_defender_node.simps(1) play_def 
           plays_for_0strategy.p1move) 
-    hence \<open>\<exists>n1'. c_set_game_moves n0 n1' \<and> n1'#n0#play \<in> plays_for_0strategy f (AttackerNode p00 {q00})\<close>
+    hence \<open>\<exists>n1'. c_set_game_moves n0 n1'
+        \<and> n1'#n0#play \<in> plays_for_0strategy f (AttackerNode p00 {q00})\<close>
       using assms(2) n0_def sound_0strategy_def
       by (meson c_set_game_defender_node.simps(3) plays_for_0strategy.p0move) 
     then obtain n1' where n1'_mov: \<open>c_set_game_moves n0 n1'\<close> 
       and in_play: \<open>n1'#n0#play \<in> plays_for_0strategy f (AttackerNode p00 {q00})\<close> by auto
     hence \<open>\<exists>q1. n1' = AttackerNode q1 {p1} \<and> (q1 \<in> weak_tau_succs {q})\<close>
-      by (metis c_set_game_defender_node.elims(2, 3) c_set_game_moves_no_step(3, 4) swap_answer n0_def) 
+      by (metis c_set_game_defender_node.elims(2, 3) c_set_game_moves_no_step(3, 4)
+          swap_answer n0_def) 
     then obtain q1 where q1_def: \<open>n1' = AttackerNode q1 {p1}\<close> 
       and q_succ: \<open>q1 \<in> weak_tau_succs {q}\<close> by auto
     hence q_tau: \<open>q \<Rightarrow>^\<tau> q1\<close> using weak_tau_succs_def by auto
@@ -523,40 +615,48 @@ proof (safe)
     case (snoc as a)
     hence \<open>A \<noteq> []\<close> by auto
     hence \<open>\<not>tau a\<close> using \<open>\<forall>a\<in>set A. a \<noteq> \<tau>\<close> snoc  by (simp add: tau_def) 
-    then obtain A_play p0 where 
-     gotoA: \<open>DefenderSimNode (last A) p0 (dsuccs_seq_rec (rev (butlast A)) {q}) # A_play
-        \<in> plays_for_0strategy f (AttackerNode p00 {q00})\<close> \<open>word_reachable_via_delay A p p0 p1\<close> 
-        using def_sim_pos_with_prefix_in_play \<open>p \<Rightarrow>$A p1\<close> 
+    then obtain A_play p0 where gotoA:
+      \<open>DefenderSimNode (last A) p0 (dsuccs_seq_rec (rev (butlast A)) {q}) # A_play
+        \<in> plays_for_0strategy f (AttackerNode p00 {q00})\<close>
+      \<open>word_reachable_via_delay A p p0 p1\<close> 
+      using def_sim_pos_with_prefix_in_play \<open>p \<Rightarrow>$A p1\<close> 
         \<open>\<forall>a\<in>set A. a \<noteq> \<tau>\<close> \<open>A \<noteq> []\<close> assms(2) play_def play_hd by meson
     then obtain Q where \<open>Q = dsuccs_seq_rec (rev (butlast A)) {q}\<close> by auto
-    hence \<open>\<forall>q' \<in> Q.  q \<Rightarrow>$(butlast A) q'\<close> using in_dsuccs_implies_word_reachable by auto
-    then obtain n0 where n0_def: \<open>n0 = DefenderSimNode a p0 (dsuccs_seq_rec (rev as) {q}) \<close> by auto
-    hence A_play_def: \<open>n0#A_play \<in> plays_for_0strategy f (AttackerNode p00 {q00})\<close> using gotoA snoc by auto
+    hence \<open>\<forall>q' \<in> Q.  q \<Rightarrow>$(butlast A) q'\<close>
+      using in_dsuccs_implies_word_reachable by auto
+    then obtain n0 where
+      n0_def: \<open>n0 = DefenderSimNode a p0 (dsuccs_seq_rec (rev as) {q})\<close>
+      by auto
+    hence A_play_def: \<open>n0#A_play \<in> plays_for_0strategy f (AttackerNode p00 {q00})\<close>
+      using gotoA snoc by auto
     then obtain n1 where n1_move: \<open>c_set_game_moves n0 n1\<close>
-      using n0_def by (meson assms(2) c_set_game_defender_node.simps(2) sound_0strategy_def)
+      using n0_def
+      by (meson assms(2) c_set_game_defender_node.simps(2) sound_0strategy_def)
     hence \<open>n1 = AttackerNode p0 (dsuccs a (dsuccs_seq_rec (rev as) {q}))\<close> 
       using move_DefSim_to_AtkNode n0_def by blast
     hence \<open>n1 = AttackerNode p0 (dsuccs_seq_rec (a#(rev as)) {q})\<close>  
       using dsuccs_seq_rec.simps(2) by auto
     hence \<open>n1 = AttackerNode p0 (dsuccs_seq_rec (rev (as@[a])) {q})\<close> by auto
-    hence n1_def: \<open>n1 = AttackerNode p0 (dsuccs_seq_rec (rev A) {q})\<close> using snoc by auto
+    hence n1_def: \<open>n1 = AttackerNode p0 (dsuccs_seq_rec (rev A) {q})\<close>
+      using snoc by auto
     hence n1_in_play: \<open>n1#n0#A_play \<in> plays_for_0strategy f (AttackerNode p00 {q00})\<close>
-      using n0_def A_play_def n1_move assms(2) move_DefSim_to_AtkNode 
-        plays_for_0strategy.p0move sound_0strategy_def 
-      by fastforce 
-    from \<open>word_reachable_via_delay A p p0 p1\<close> have \<open>p0 \<Rightarrow>^\<tau> p1\<close> 
+      using n0_def A_play_def n1_move assms(2) move_DefSim_to_AtkNode
+        plays_for_0strategy.p0move sound_0strategy_def
+      by fastforce
+    from \<open>word_reachable_via_delay A p p0 p1\<close> have \<open>p0 \<Rightarrow>^\<tau> p1\<close>
       using word_reachable_via_delay_def by auto
     then obtain n0' where n0'_move: \<open>c_set_game_moves n1 n0'\<close>
       and n0'_def: \<open>n0' = DefenderSwapNode p1 (dsuccs_seq_rec (rev A) {q})\<close>
       using  swap_challenge tau_tau n1_def by blast
-    hence n0'_in_play: \<open>n0'#n1#n0#A_play \<in> plays_for_0strategy f (AttackerNode p00 {q00})\<close>
+    hence n0'_in_play:
+      \<open>n0'#n1#n0#A_play \<in> plays_for_0strategy f (AttackerNode p00 {q00})\<close>
       using n1_in_play by (simp add: n1_def plays_for_0strategy.p1move) 
     then obtain n1' where n1'_move: \<open>c_set_game_moves n0' n1'\<close>
       and in_strat: \<open>n1' = f(n0'#n1#n0#A_play)\<close> 
       using Def_not_stuck n0'_def assms(2) sound_0strategy_def by auto
     then obtain q1 where q1_def: \<open>q1 \<in> weak_tau_succs (dsuccs_seq_rec (rev A) {q})\<close> 
-      and n1'_def: \<open>n1'  = AttackerNode q1 {p1}\<close> using n0'_def
-      by (metis c_set_game_defender_node.cases c_set_game_moves_no_step(3, 7) swap_answer) 
+      and n1'_def: \<open>n1'  = AttackerNode q1 {p1}\<close> using n0'_def swap_answer
+      by (metis c_set_game_defender_node.cases c_set_game_moves_no_step(3, 7)) 
     hence \<open>q1 \<in> {q1. \<exists>q0 \<in> (dsuccs_seq_rec (rev A) {q}). q0 \<Rightarrow>^\<tau> q1}\<close> 
       using weak_tau_succs_def by auto
     also have \<open>... = {q1. \<exists>q0 \<in> (dsuccs_seq_rec (rev A) {q}). q \<Rightarrow>$A q0 \<and> q0 \<Rightarrow>^\<tau> q1}\<close>
@@ -566,32 +666,39 @@ proof (safe)
     also have \<open>... \<subseteq> {q1. q \<Rightarrow>$A q1}\<close> by auto
     finally have \<open>q1 \<in> {q1. q \<Rightarrow>$A q1}\<close> .
     hence q_goal: \<open>q \<Rightarrow>$A q1\<close> by auto
-    from n1'_move in_strat have move_f: \<open>c_set_game_moves n0' (f(n0'#n1#n0#A_play))\<close> by auto
-    hence  \<open>n1'#n0'#n1#n0#A_play \<in> plays_for_0strategy f (AttackerNode p00 {q00})\<close>
+    from n1'_move in_strat have
+      move_f: \<open>c_set_game_moves n0' (f(n0'#n1#n0#A_play))\<close> by auto
+    hence \<open>n1'#n0'#n1#n0#A_play \<in> plays_for_0strategy f (AttackerNode p00 {q00})\<close>
       using in_strat plays_for_0strategy.p0move[OF n0'_in_play _ move_f] n0'_def by auto
-    hence \<open>C q1 p1\<close> unfolding C_def using n1'_def n0'_def by force 
+    hence \<open>C q1 p1\<close> unfolding C_def using n1'_def n0'_def by force
     thus ?thesis using q_goal by auto
   qed
 qed
 
 theorem winning_strategy_in_set_game_iff_contrasim:
-  shows 
-    \<open>(\<exists> f . player0_winning_strategy f (AttackerNode p0 {q0}) \<and> sound_0strategy f (AttackerNode p0 {q0}))
+  shows
+    \<open>(\<exists> f . player0_winning_strategy f (AttackerNode p0 {q0})
+      \<and> sound_0strategy f (AttackerNode p0 {q0}))
     = p0 \<sqsubseteq>c q0\<close>
 proof safe
   fix f
-  assume \<open>player0_winning_strategy f (AttackerNode p0 {q0})\<close> \<open>sound_0strategy f (AttackerNode p0 {q0})\<close>
+  assume
+    \<open>player0_winning_strategy f (AttackerNode p0 {q0})\<close>
+    \<open>sound_0strategy f (AttackerNode p0 {q0})\<close>
   hence \<open>contrasimulation (\<lambda>p q. \<exists>play \<in> plays_for_0strategy f (AttackerNode p0 {q0}).
-                 hd play = AttackerNode p {q} \<and>
-                 (hd play = (AttackerNode p0 {q0}) \<or> (\<exists>P. hd (tl play) = DefenderSwapNode q P)))\<close>
+    hd play = AttackerNode p {q} \<and>
+    (hd play = (AttackerNode p0 {q0}) \<or> (\<exists>P. hd (tl play) = DefenderSwapNode q P)))\<close>
     using set_contrasim_game_sound by blast
-  thus  \<open>p0 \<sqsubseteq>c q0\<close> using plays_for_0strategy.init[of \<open>AttackerNode p0 {q0}\<close> f] list.sel(1) by force
+  thus \<open>p0 \<sqsubseteq>c q0\<close>
+    using plays_for_0strategy.init[of \<open>AttackerNode p0 {q0}\<close> f] list.sel(1) by force
 next
   fix C
   assume \<open>contrasimulation C\<close> \<open>C p0 q0\<close>
-  thus \<open>(\<exists>f. player0_winning_strategy f (AttackerNode p0 {q0}) \<and> sound_0strategy f (AttackerNode p0 {q0}))\<close>
-    using set_contrasim_game_complete[OF _ _]
-         strategy_from_mimicking_of_C_sound[OF _ _] by blast
+  thus
+    \<open>(\<exists>f. player0_winning_strategy f (AttackerNode p0 {q0})
+      \<and> sound_0strategy f (AttackerNode p0 {q0}))\<close>
+    using set_contrasim_game_complete[OF _ _] strategy_from_mimicking_of_C_sound[OF _ _]
+    by blast
 qed
 
 end
