Simple_Game.thy
@@ -15,8 +15,9 @@ begin
 abbreviation player1_position :: \<open>'s \<Rightarrow> bool\<close>
   where \<open>player1_position s \<equiv> \<not> player0_position s\<close>
 
-\<comment>\<open>plays (to be precise: play prefixes) are lists. we model them 
-  with the most recent move at the beginning. (for our purpose it's enough to consider finite plays)\<close>
+\<comment>\<open>Plays (to be precise: play prefixes) are lists.
+  We model them with the most recent move at the beginning.
+  (For our purpose it's enough to consider finite plays.)\<close>
 type_synonym ('s2) play = \<open>'s2 list\<close>
 type_synonym ('s2) strategy = \<open>'s2 play \<Rightarrow> 's2\<close>
 type_synonym ('s2) posstrategy = \<open>'s2 \<Rightarrow> 's2\<close>
@@ -32,13 +33,15 @@ inductive_set plays :: \<open>'s \<Rightarrow> 's play set\<close>
 definition play_continuation :: \<open>'s play \<Rightarrow> 's play \<Rightarrow> bool\<close>
   where \<open>play_continuation p1 p2 \<equiv> (drop (length p2 - length p1) p2) = p1\<close>
 
-\<comment>\<open>plays for a given player 0 strategy\<close>
+\<comment>\<open>Plays for a given player 0 strategy\<close>
 inductive_set plays_for_0strategy :: \<open>'s strategy \<Rightarrow> 's \<Rightarrow> 's play set\<close>
   for f initial where
   init: \<open>[initial] \<in> plays_for_0strategy f initial\<close> |
-  p0move: \<open>n0#play \<in> plays_for_0strategy f initial \<Longrightarrow> player0_position n0 \<Longrightarrow> n0 \<longmapsto>\<heartsuit> f (n0#play)
+  p0move:
+    \<open>n0#play \<in> plays_for_0strategy f initial \<Longrightarrow> player0_position n0 \<Longrightarrow> n0 \<longmapsto>\<heartsuit> f (n0#play)
     \<Longrightarrow> (f (n0#play))#n0#play \<in> plays_for_0strategy f initial\<close> |
-  p1move: \<open>n1#play \<in> plays_for_0strategy f initial \<Longrightarrow> player1_position n1 \<Longrightarrow> n1 \<longmapsto>\<heartsuit> n1'
+  p1move:
+    \<open>n1#play \<in> plays_for_0strategy f initial \<Longrightarrow> player1_position n1 \<Longrightarrow> n1 \<longmapsto>\<heartsuit> n1'
     \<Longrightarrow> n1'#n1#play \<in> plays_for_0strategy f initial\<close>
 
 lemma strategy0_step:
@@ -50,27 +53,32 @@ lemma strategy0_step:
   using assms
   by (induct rule: plays_for_0strategy.cases, auto)
 
-\<comment>\<open>plays for a given player 1 strategy\<close>
+\<comment>\<open>Plays for a given player 1 strategy\<close>
 inductive_set plays_for_1strategy :: \<open>'s strategy \<Rightarrow> 's \<Rightarrow> 's play set\<close>
   for f initial where
   init: \<open>[initial] \<in> plays_for_1strategy f initial\<close> |
-  p0move: \<open>n0#play \<in> plays_for_1strategy f initial \<Longrightarrow> player0_position n0 \<Longrightarrow> n0 \<longmapsto>\<heartsuit> n0'
+  p0move:
+    \<open>n0#play \<in> plays_for_1strategy f initial \<Longrightarrow> player0_position n0 \<Longrightarrow> n0 \<longmapsto>\<heartsuit> n0'
     \<Longrightarrow> n0'#n0#play \<in> plays_for_1strategy f initial\<close> |
-  p1move: \<open>n1#play \<in> plays_for_1strategy f initial \<Longrightarrow> player1_position n1 \<Longrightarrow> n1 \<longmapsto>\<heartsuit> f (n1#play)
+  p1move:
+    \<open>n1#play \<in> plays_for_1strategy f initial \<Longrightarrow> player1_position n1 \<Longrightarrow> n1 \<longmapsto>\<heartsuit> f (n1#play)
     \<Longrightarrow> (f (n1#play))#n1#play \<in> plays_for_1strategy f initial\<close>
-
 
 definition positional_strategy :: \<open>'s strategy \<Rightarrow> bool\<close> where
   \<open>positional_strategy f \<equiv> \<forall>r1 r2 n. f (n # r1) = f (n # r2)\<close>
 
-text \<open>a strategy is sound if it only decides on enabled transitions.\<close>
+text \<open>A strategy is sound if it only decides on enabled transitions.\<close>
 definition sound_0strategy :: \<open>'s strategy \<Rightarrow> 's \<Rightarrow> bool\<close> where
   \<open>sound_0strategy f initial \<equiv>
-    \<forall> n0 play . n0#play \<in> plays_for_0strategy f initial \<and> player0_position n0 \<longrightarrow> n0 \<longmapsto>\<heartsuit> f (n0#play)\<close>
+    \<forall> n0 play .
+      n0#play \<in> plays_for_0strategy f initial \<and>
+      player0_position n0 \<longrightarrow> n0 \<longmapsto>\<heartsuit> f (n0#play)\<close>
 
 definition sound_1strategy :: \<open>'s strategy \<Rightarrow> 's \<Rightarrow> bool\<close> where
   \<open>sound_1strategy f initial \<equiv>
-    \<forall> n1 play . n1#play \<in> plays_for_1strategy f initial \<and> player1_position n1 \<longrightarrow> n1 \<longmapsto>\<heartsuit> f (n1#play)\<close>
+    \<forall> n1 play .
+      n1#play \<in> plays_for_1strategy f initial \<and>
+      player1_position n1 \<longrightarrow> n1 \<longmapsto>\<heartsuit> f (n1#play)\<close>
 
 lemma strategy0_plays_subset:
   assumes \<open>play \<in> plays_for_0strategy f initial\<close>
@@ -86,13 +94,14 @@ lemma no_empty_plays:
   shows \<open>False\<close> 
   using assms plays.cases by blast
 
-text \<open>player1 wins a play if the play has reached a deadlock where it's player0's turn\<close>
+text \<open>Player1 wins a play if the play has reached a deadlock where it's player0's turn\<close>
 
 definition player1_wins_immediately :: \<open>'s play \<Rightarrow> bool\<close> where
   \<open>player1_wins_immediately play \<equiv> player0_position (hd play) \<and> (\<nexists> p' . (hd play) \<longmapsto>\<heartsuit> p')\<close>
 
 definition player0_winning_strategy :: \<open>'s strategy \<Rightarrow> 's \<Rightarrow> bool\<close> where
-  \<open>player0_winning_strategy f initial \<equiv> (\<forall> play \<in> plays_for_0strategy f initial . \<not> player1_wins_immediately play)\<close>
+  \<open>player0_winning_strategy f initial \<equiv> (\<forall> play \<in> plays_for_0strategy f initial.
+    \<not> player1_wins_immediately play)\<close>
 
 definition player0_wins :: \<open>'s \<Rightarrow> bool\<close> where
   \<open>player0_wins s \<equiv> (\<exists> f . player0_winning_strategy f s \<and> sound_0strategy f s)\<close>
@@ -112,55 +121,8 @@ proof -
         sound_0strategy_def strategy0_plays_subset)
 qed
 
-
 definition player0_wins_immediately :: \<open>'s play \<Rightarrow> bool\<close> where
   \<open>player0_wins_immediately play \<equiv> player1_position (hd play) \<and> (\<nexists> p' . (hd play) \<longmapsto>\<heartsuit> p')\<close>
 
-
-\<comment> \<open>in comparison to the defender, the attacker also has to bound the depth of plays.\<close>
-definition player1_winning_strategy :: \<open>'s strategy \<Rightarrow> 's \<Rightarrow> bool\<close> where
-  \<open>player1_winning_strategy f initial \<equiv>
-    \<exists>maxn. (\<forall> play \<in> plays_for_1strategy f initial . \<not> player0_wins_immediately play \<and> length play \<le> maxn)\<close>
-
-definition player1_wins :: \<open>'s \<Rightarrow> bool\<close> where
-  \<open>player1_wins s \<equiv> (\<exists> f . player1_winning_strategy f s \<and> sound_1strategy f s)\<close>
-
-
-
-lemma stuck_0_all_strats_win:
-  assumes \<open>player0_position initial\<close> \<open>(\<nexists> p' . initial \<longmapsto>\<heartsuit> p')\<close>
-  shows  \<open>\<forall>f. player1_winning_strategy f initial\<close>
-proof -
-  have \<open>\<And>pl. pl \<in> plays initial \<Longrightarrow> pl = [initial]\<close>
-  proof -
-    fix pl
-    assume \<open>pl \<in> plays initial\<close>
-    thus \<open>pl = [initial]\<close> using assms(2) by (induct, auto)
-  qed
-  hence \<open>\<forall>f. (\<forall> play \<in> plays_for_1strategy f initial . \<not> player0_wins_immediately play \<and> length play \<le> 1)\<close>
-    by (metis assms(1) butlast.simps(1) butlast_conv_take diff_is_0_eq' 
-       le_numeral_extra(4) length_tl list.sel(1, 2) list.size(3) 
-       one_eq_numeral_iff player0_wins_immediately_def 
-       strategy1_plays_subset take_Cons_numeral take_all_iff)
-  thus ?thesis using player1_winning_strategy_def by auto
-qed
-
-lemma stuck_player1_win:
- assumes \<open>player0_position initial\<close> \<open>(\<nexists> p' . initial \<longmapsto>\<heartsuit> p')\<close>
-  shows \<open>player1_wins initial\<close>
-proof -
-  have all_plays_stuck: \<open>\<And>pl. pl \<in> plays initial \<Longrightarrow> pl = [initial]\<close>
-  proof -
-    fix pl
-    assume \<open>pl \<in> plays initial\<close>
-    thus \<open>pl = [initial]\<close> using assms(2) by (induct, auto)
-  qed
-  have \<open>sound_1strategy (\<lambda>x. hd x) initial\<close> 
-    unfolding sound_1strategy_def 
-    using all_plays_stuck assms(1) strategy1_plays_subset by auto
-  thus ?thesis unfolding player1_wins_def using assms stuck_0_all_strats_win by auto
-qed
-
 end
-
 end
